bedrock2/src/bedrock2/NotationsCustomEntry.v
@@ -1,6 +1,9 @@
 Require Import Coq.ZArith.BinIntDef Coq.Strings.String.
 Require Import coqutil.Macros.subst coqutil.Macros.unique bedrock2.Syntax.
-Export Syntax.Coercions.
+
+Export Coq.Strings.String.StringSyntax.
+Export bedrock2.Syntax.Coercions.
+Number Notation BinInt.Z BinInt.Z.of_num_int BinInt.Z.to_num_int : Z_scope.
 
 (** Grammar for expressions *)
 
