bedrock2/src/bedrock2Examples/ARPResponder.v
@@ -4,69 +4,66 @@ Require Import bedrock2.FE310CSemantics.
 
 Import Syntax BinInt String List.ListNotations ZArith.
 Local Open Scope string_scope. Local Open Scope Z_scope. Local Open Scope list_scope.
-Local Coercion expr.literal : Z >-> expr.
-Local Coercion expr.var : String.string >-> expr.
-Local Coercion name_of_func (f : function) : String.string := fst f.
 
 Definition arp : bedrock_func :=
     let ethbuf : String.string := "ethbuf" in
     let buf : String.string := "buf" in
     let len : String.string := "len" in
   ("arp", ([ethbuf; len], [], bedrock_func_body:(
-    require ( coq:(14+27) < len ) else { /*skip*/ };
-    require ( (load1(ethbuf+coq:(14+0))== coq:(0))
-            & (load1(ethbuf+coq:(14+1)) == coq:(1))
-            & (load1(ethbuf+coq:(14+2)) == coq:(0x08))
-            & (load1(ethbuf+coq:(14+3)) == coq:(0))
-            & (load1(ethbuf+coq:(14+4)) == coq:(6))
-            & (load1(ethbuf+coq:(14+5)) == coq:(4))
+    require ( $(14+27) < len ) else { /*skip*/ };
+    require ( (load1(ethbuf+$(14+0))== $0)
+            & (load1(ethbuf+$(14+1)) == $1)
+            & (load1(ethbuf+$(14+2)) == $0x08)
+            & (load1(ethbuf+$(14+3)) == $0)
+            & (load1(ethbuf+$(14+4)) == $6)
+            & (load1(ethbuf+$(14+5)) == $4)
             ) else { /*skip*/ };
     (* TODO: update sender mapping if present *)
-    require ( (load1(ethbuf+coq:(14+6)) == coq:(0))
-            & (load1(ethbuf+coq:(14+6+1)) == coq:(1))
+    require ( (load1(ethbuf+$(14+6)) == $0)
+            & (load1(ethbuf+$(14+6+1)) == $1)
             ) else { /*skip*/ }; (* request *)
-    store1(ethbuf+coq:(14+6+1), coq:(2)); (* response *)
+    store1(ethbuf+$(14+6+1), $2); (* response *)
     (* TODO: add sender mapping to arp table *)
 
     (* dst := src *)
-    store1(ethbuf+coq:(14+18  ), load1(ethbuf+coq:(14+8  )));
-    store1(ethbuf+coq:(14+18+1), load1(ethbuf+coq:(14+8+1)));
-    store1(ethbuf+coq:(14+18+2), load1(ethbuf+coq:(14+8+2)));
-    store1(ethbuf+coq:(14+18+3), load1(ethbuf+coq:(14+8+3)));
-    store1(ethbuf+coq:(14+18+4), load1(ethbuf+coq:(14+8+4)));
-    store1(ethbuf+coq:(14+18+5), load1(ethbuf+coq:(14+8+5)));
-    store1(ethbuf+coq:(14+18+6), load1(ethbuf+coq:(14+8+6)));
-    store1(ethbuf+coq:(14+18+7), load1(ethbuf+coq:(14+8+7)));
-    store1(ethbuf+coq:(14+18+8), load1(ethbuf+coq:(14+8+8)));
-    store1(ethbuf+coq:(14+18+9), load1(ethbuf+coq:(14+8+9)));
+    store1(ethbuf+$(14+18  ), load1(ethbuf+$(14+8  )));
+    store1(ethbuf+$(14+18+1), load1(ethbuf+$(14+8+1)));
+    store1(ethbuf+$(14+18+2), load1(ethbuf+$(14+8+2)));
+    store1(ethbuf+$(14+18+3), load1(ethbuf+$(14+8+3)));
+    store1(ethbuf+$(14+18+4), load1(ethbuf+$(14+8+4)));
+    store1(ethbuf+$(14+18+5), load1(ethbuf+$(14+8+5)));
+    store1(ethbuf+$(14+18+6), load1(ethbuf+$(14+8+6)));
+    store1(ethbuf+$(14+18+7), load1(ethbuf+$(14+8+7)));
+    store1(ethbuf+$(14+18+8), load1(ethbuf+$(14+8+8)));
+    store1(ethbuf+$(14+18+9), load1(ethbuf+$(14+8+9)));
 
     (* eth_dst = src *)
-    store1(ethbuf           , load1(ethbuf+coq:(14+8  )));
-    store1(ethbuf+coq:(1), load1(ethbuf+coq:(14+8+1)));
-    store1(ethbuf+coq:(2), load1(ethbuf+coq:(14+8+2)));
-    store1(ethbuf+coq:(3), load1(ethbuf+coq:(14+8+3)));
-    store1(ethbuf+coq:(4), load1(ethbuf+coq:(14+8+4)));
-    store1(ethbuf+coq:(5), load1(ethbuf+coq:(14+8+5)));
+    store1(ethbuf           , load1(ethbuf+$(14+8  )));
+    store1(ethbuf+$1, load1(ethbuf+$(14+8+1)));
+    store1(ethbuf+$2, load1(ethbuf+$(14+8+2)));
+    store1(ethbuf+$3, load1(ethbuf+$(14+8+3)));
+    store1(ethbuf+$4, load1(ethbuf+$(14+8+4)));
+    store1(ethbuf+$5, load1(ethbuf+$(14+8+5)));
 
     (* src := me *)
-    store1(ethbuf+coq:(14+8  ), coq:(0xf0));
-    store1(ethbuf+coq:(14+8+1), coq:(0xf1));
-    store1(ethbuf+coq:(14+8+2), coq:(0xf2));
-    store1(ethbuf+coq:(14+8+3), coq:(0xf3));
-    store1(ethbuf+coq:(14+8+4), coq:(0xf4));
-    store1(ethbuf+coq:(14+8+5), coq:(0xf5));
-    store1(ethbuf+coq:(14+8+6), coq:( 10));
-    store1(ethbuf+coq:(14+8+7), coq:(155));
-    store1(ethbuf+coq:(14+8+8), coq:(  5));
-    store1(ethbuf+coq:(14+8+9), coq:(  1));
+    store1(ethbuf+$(14+8  ), $0xf0);
+    store1(ethbuf+$(14+8+1), $0xf1);
+    store1(ethbuf+$(14+8+2), $0xf2);
+    store1(ethbuf+$(14+8+3), $0xf3);
+    store1(ethbuf+$(14+8+4), $0xf4);
+    store1(ethbuf+$(14+8+5), $0xf5);
+    store1(ethbuf+$(14+8+6), $ 10);
+    store1(ethbuf+$(14+8+7), $155);
+    store1(ethbuf+$(14+8+8), $  5);
+    store1(ethbuf+$(14+8+9), $  1);
 
     (* eth_src = me *)
-    store1(ethbuf+coq:(6+0), coq:(0xf0));
-    store1(ethbuf+coq:(6+1), coq:(0xf1));
-    store1(ethbuf+coq:(6+2), coq:(0xf2));
-    store1(ethbuf+coq:(6+3), coq:(0xf3));
-    store1(ethbuf+coq:(6+4), coq:(0xf4));
-    store1(ethbuf+coq:(6+5), coq:(0xf5));
+    store1(ethbuf+$(6+0), $0xf0);
+    store1(ethbuf+$(6+1), $0xf1);
+    store1(ethbuf+$(6+2), $0xf2);
+    store1(ethbuf+$(6+3), $0xf3);
+    store1(ethbuf+$(6+4), $0xf4);
+    store1(ethbuf+$(6+5), $0xf5);
 
     /*skip*/
 ))).
@@ -85,12 +82,12 @@ Definition ethernet : bedrock_func :=
     let len : String.string := "len" in
     let ethertype : String.string := "ethertype" in
   ("ethernet", ((buf::len::nil), @nil String.string, bedrock_func_body:(
-    require (coq:(14) < len) else { /*skip*/ } ;
-    ethertype = (load1(buf + coq:(12)) << coq:(8)) | (load1(buf + coq:(13)));
-    require (coq:(0x600-1) < ethertype) else { /*skip*/ };
-    if (ethertype == coq:(0x0800)) {
-      ipv4(buf+coq:(14), len-coq:(14))
-    } else if (ethertype == coq:(0x0806)) {
+    require ($14 < len) else { /*skip*/ } ;
+    ethertype = (load1(buf + $12) << $8) | (load1(buf + $13));
+    require ($(0x600-1) < ethertype) else { /*skip*/ };
+    if (ethertype == $0x0800) {
+      ipv4(buf+$14, len-$14)
+    } else if (ethertype == $0x0806) {
       arp(buf, len)
     }
 ))).
